Batched GEMM supporting arbitrary comb binop

dist/Klas_GEMM_Batched.h
@@ -4,11 +4,19 @@
 
 #include <kuiper.h>
 
+void
+Klas_GEMM_Batched_batched_gemm_f32(float alpha,
+                                   float beta,
+                                   uint32_t batch,
+                                   uint32_t rows,
+                                   uint32_t shared,
+                                   uint32_t cols, float *a, float *b, float *c);
+
 float
-*Klas_GEMM_Batched_batched_gemm_f32(uint32_t batch,
-                                    uint32_t rows,
-                                    uint32_t shared,
-                                    uint32_t cols, float *a, float *b);
+*Klas_GEMM_Batched_batched_matmul_f32(uint32_t batch,
+                                      uint32_t rows,
+                                      uint32_t shared,
+                                      uint32_t cols, float *a, float *b);
 
 #define Klas_GEMM_Batched_H_DEFINED
 #endif                          /* Klas_GEMM_Batched_H */
