src/klas/Klas.GEMM.Batched.fst
@@ -3,5 +3,48 @@ module Klas.GEMM.Batched
 #lang-pulse
 open Kuiper
 module K = Kuiper.Kernel.BatchedGEMM
+open Kuiper.Tensor.Layout.Alg
+module Array3 = Kuiper.Array3
+module EM = Kuiper.EMatrix
+module EMatrix3 = Kuiper.EMatrix3
+module MS = Kuiper.Spec.GEMM
+module SZ = Kuiper.SizeT
 
-let batched_gemm_f32 = K.batched_gemm_f32
+inline_for_extraction noextract
+fn batched_matmul
+  (#et : Type0) {| scalar et |}
+  (batch rows shared cols : szp)
+  (a : Array3.t et (l3_batched_row_major batch rows shared) { Array3.is_global a })
+  (b : Array3.t et (l3_batched_row_major batch shared cols) { Array3.is_global b })
+  (#sa : erased (EMatrix3.t et batch rows shared))
+  (#sb : erased (EMatrix3.t et batch shared cols))
+  (#fA #fB : perm)
+  norewrite
+  preserves
+    cpu **
+    on gpu_loc (a |-> Frac fA sa) **
+    on gpu_loc (b |-> Frac fB sb)
+  requires
+    pure (
+      rows * cols <= max_blocks * max_threads  /\
+      SZ.fits (batch * rows * cols)
+    )
+  returns
+    out : Array3.t et (l3_batched_row_major batch rows cols)
+  ensures
+    on gpu_loc (out |-> MS.batched_matmul sa sb) **
+    pure (Array3.is_global out)
+{
+  let out = Array3.alloc0 #et batch rows cols (l3_batched_row_major batch rows cols);
+  with sc0. assert on gpu_loc (out |-> sc0);
+  K.bmmcomb_gpu_exact #et (MS.comb2) batch rows shared cols a b out #sa #sb #sc0 #fA #fB;
+  out
+}
+
+inline_for_extraction noextract
+let batched_gemm 
+  (#et : Type0) {| scalar et |} 
+  (alpha beta : et) = K.bmmcomb_gpu_exact #et (MS.lincomb alpha beta)
+
+let batched_gemm_f32 = batched_gemm #f32
+let batched_matmul_f32 = batched_matmul #f32
