src/lib/spec/Kuiper.Spec.GEMM.fsti
@@ -7,6 +7,8 @@ open Kuiper
 open Kuiper.EMatrix
 open Kuiper.EMatrix.Tiling
 
+module EM3 = Kuiper.EMatrix3
+
 inline_for_extraction noextract
 let comb2 (#et:Type) (x y : et) : et = y
 
@@ -391,3 +393,35 @@ val matmul_tiles_lemma
         (ematrix_subtile m1 trows shared i 0)
         (ematrix_subtile m2 shared tcols 0 j)
     ))
+
+(* Per-page batched gemm spec. *)
+let bmmcomb
+  (#et:Type) {| scalar et |}
+  (comb : binop et)
+  (#batch #rows #shared #cols : nat)
+  (c : EM3.t et batch rows cols)
+  (a : EM3.t et batch rows shared)
+  (b : EM3.t et batch shared cols)
+  : EM3.t et batch rows cols
+  = EM3.mkM fun i j k ->
+      macc (mmcomb comb (EM3.slice_page c i) (EM3.slice_page a i) (EM3.slice_page b i)) j k
+
+(* Per-page batched matmul spec. *)
+let batched_matmul
+  (#et:Type) {| scalar et |}
+  (#batch #rows #shared #cols : nat)
+  (a : EM3.t et batch rows shared)
+  (b : EM3.t et batch shared cols)
+  : EM3.t et batch rows cols
+  = EM3.mkM fun i j k ->
+      macc (matmul (EM3.slice_page a i)
+                         (EM3.slice_page b i)) j k
+
+val bmatmul_is_bgemm
+  (#et:Type) {| scalar et |}
+  (#batch #rows #shared #columns : nat)
+  (m0 : EM3.t et batch rows columns)
+  (m1 : EM3.t et batch rows shared)
+  (m2 : EM3.t et batch shared columns)
+  : Lemma (bmmcomb comb2 m0 m1 m2 == batched_matmul m1 m2)
+          [SMTPat (bmmcomb comb2 m0 m1 m2)]
